Left Pi2, proved confluence and injectivity of Pi :))

proof/TPOSR/ChurchRosser.v
@@ -1,3 +1,4 @@
+
 Require Import Lambda.Utils.
 Require Import Lambda.Tactics.
 Require Import Lambda.MyList.
@@ -18,1051 +19,266 @@ Require Import TPOSR.Generation.
 Require Import TPOSR.TypesDepth.
 Require Import TPOSR.TypesFunctionality.
 Require Import TPOSR.UniquenessOfTypes.
-(*Require Import TPOSR.CtxConversionDepth.*)
-
+Require Import TPOSR.ChurchRosserDepth.
 
 Require Import Meta.TPOSR_Russell.
 
-Require Import TPOSR.MaxLemmas.
-
 Set Implicit Arguments.
 
-Definition tod := tposr_tposrd_type.
-Definition fromd := tposrd_tposr_type.
-
-Lemma tposr_equiv_l : forall e A B, equiv e A B -> forall M N, 
-  e |-- M -> N : A -> e |-- M -> N : B.
-Proof.
-  destruct 1 ; intros.
-  rewrite <- H ; assumption.
-  destruct H.
-  apply tposr_conv_l with A x ; auto.
-Qed. 
-
-Lemma tposr_equiv_r : forall e A B, equiv e A B -> forall M N, 
-  e |-- M -> N : B -> e |-- M -> N : A.
-Proof.
-  destruct 1 ; intros.
-  rewrite H ; assumption.
-  destruct H.
-  apply tposr_conv_r with B x ; auto.
-Qed. 
-
-Theorem church_rosser : forall n m,
-  forall G M N A, G |-- M -> N : A [n] ->
-  forall P B, G |-- M -> P : B [m] ->
+Corollary church_rosser : forall G M N A, G |-- M -> N : A -> forall P B, G |-- M -> P : B ->
   exists Q, 
   (G |-- N -> Q : A /\
   G |-- N -> Q : B /\
   G |-- P -> Q : A /\
   G |-- P -> Q : B).
 Proof.
-  intros n.
-  pattern n.
+  intros.
+  pose (tod H).
+  pose (tod H0).
+  destruct_exists.
+  apply (church_rosser_depth H2 H1).
+Qed.
+
+Inductive tposrp_n : lenv -> lterm -> lterm -> lterm -> nat -> Prop :=
+  | tposrp_n_tposr : forall e X Y Z, e |-- X -> Y : Z -> tposrp_n e X Y Z 1
+  | tposrp_n_trans : forall e W X Z, e |-- W -> X : Z -> forall Y m, tposrp_n e X Y Z m ->
+  tposrp_n e W Y Z (S m).
+
+Lemma tposrp_n_tposrp :  forall e T U s n, tposrp_n e T U s n -> tposrp e T U s.
+Proof.
+  induction 1.
+  apply tposrp_tposr ; auto.
+  apply tposrp_trans with X ; auto.
+  apply tposrp_tposr ; auto.
+Qed. 
+
+Lemma tposrp_n_cr : 
+  forall n m e A B T, tposrp_n e A B T n -> forall C, tposrp_n e A C T m -> 
+  exists D, tposrp_n e B D T m /\ tposrp_n e C D T n.
+Proof.
+  intros n ; pattern n.
   apply wf_lt_induction_type.
-  intros x IH m.
+  intros n' IH.
+  intros m ; pattern m.
+  apply wf_lt_induction_type.
+  intros m' IH'.
+  induction 1 ; simpl.
+  induction 1 ; simpl.
 
-  intros G M N A Hl.
-  pose (Hl2 := fromd Hl).
-  inversion Hl.
-  rewrite <- H2 in Hl2.
-  rewrite <- H3 in Hl2.
+  pose (church_rosser H H0) ; destruct_exists.
+  exists x ; intuition.
+  apply tposrp_n_tposr ; auto.
+  apply tposrp_n_tposr ; auto.
 
-  (* Var *)
-  intros P B Hr.
-  pose (Hr2 := fromd Hr).
-  pose (generation_var Hr2) ; destruct_exists.
-  rewrite H6 in Hr2.
-  rewrite H6.
-  exists (Ref_l n0) ; intuition.
+  clear IHtposrp_n.  
+  pose (church_rosser H H0); destruct_exists.
+  assert(m0 < S m0) ; auto with arith.
+  pose (tposrp_n_tposr H4).
+  pose (IH' _ H6 _ _ _ _ t _ H1) ; destruct_exists.
+  exists x0 ; intuition.
+  apply tposrp_n_trans with x ; auto.
   
-  (* Set *)
-  intros P B Hr.
-  pose (generation_sort (fromd Hr)) ; destruct_exists.
-  rewrite H5.
-  rewrite H5 in Hr.
-  rewrite H6.
-  rewrite H6 in Hr.
-  pose (fromd Hr).
-  exists (Srt_l set) ; intuition.
+  clear IHtposrp_n.
+  induction 1 ; simpl.
+  pose (church_rosser H H1) ; destruct_exists.
+  pose (tposrp_n_tposr H2).
+  assert(m0 < S m0) ; auto with arith.
+  pose (IH _ H6 1 _ _ _ _ H0 _ (tposrp_n_tposr H2)) ; destruct_exists.
+  exists x0 ; intuition.
+  apply tposrp_n_trans with x ; auto.
 
-  (* Prop *)
-  intros P B Hr.
-  pose (generation_sort (fromd Hr)) ; destruct_exists.
-  rewrite H5.
-  rewrite H5 in Hr.
-  rewrite H6.
-  rewrite H6 in Hr.
-  pose (fromd Hr).
-  exists (Srt_l prop) ; intuition.
+  clear IHtposrp_n.
+  pose (church_rosser H H1) ; destruct_exists.
+  assert(m0 < S m0) ; auto with arith.
+  pose (IH _ H7 _ _ _ _ _ H0 _ (tposrp_n_tposr H3)) ; destruct_exists.
+  assert(m1 < S m1) ; auto with arith.
+  pose (tposrp_n_trans H6 H9).
+  pose (IH' _ H10 _ _ _ _ t _ H2) ; destruct_exists.
+  exists x1 ; intuition ; auto with coc.
+  apply tposrp_n_trans with x0 ; auto.
+  inversion H8.
+  assumption.
+  inversion_clear H19.
+Qed.
 
-  (* Prod *)
-  rewrite <- H2 in Hl2.
-  rewrite <- H3 in Hl2.
-  rewrite <- H4 in Hl2.
-  intros P B0 Hr.
-  pose (generation_prod Hr) ; destruct_exists.
-  rewrite H10.
+Lemma tposrp_n_transitive : forall e T U s n, tposrp_n e T U s n -> forall V m, tposrp_n e U V s m ->
+  tposrp_n e T V s (n + m).
+Proof.
+  induction 1 ; intros.
+  simpl.
+  apply tposrp_n_trans with Y ; auto.
+  pose (IHtposrp_n V m0 H1).
+  change (S m + m0) with (S (m + m0)).
+  apply tposrp_n_trans with X ; auto with coc.
+Qed.
 
-  assert(n0 < x) ; try rewrite <- H5 ; auto with arith.
-  pose (IH _ H12 _ _ _ _ _ H _ _ H6) ; destruct_exists.
-  assert(m0 < x) ; try rewrite <- H5 ; auto with arith.
-  pose (IH _ H17 _ _ _ _ _ H0 _ _ H8) ; destruct_exists.
-  assert(conv_in_env (A0 :: G) (A' :: G)).
-  apply conv_env_hd with s1 ; auto with coc.
-  apply tposr_eq_tposr ; apply (fromd H).
-  assert(conv_in_env (A0 :: G) (a :: G)).
-  apply conv_env_hd with b ; auto with coc.
-  apply tposr_eq_tposr ; apply (fromd H6).
 
-  exists (Prod_l x0 x1) ; intuition ; try apply tposr_prod with s1 ; 
-  try apply tposr_prod with b ; auto with coc.
-  apply conv_env with (A0 :: G) ; auto with coc.
-  apply tposr_equiv_r with (Srt_l b0) ; auto.
-  apply tposr_prod with s1 ; auto with coc.
-  apply conv_env with (A0 :: G) ; auto with coc.
-  apply conv_env with (A0 :: G) ; auto with coc.
-  apply tposr_equiv_r with (Srt_l b0) ; auto.
-  apply tposr_prod with s1 ; auto with coc.
-  apply conv_env with (A0 :: G) ; auto with coc.
+Lemma tposrp_tposrp_n : forall e T U s, tposrp e T U s -> exists n, tposrp_n e T U s n.
+Proof.
+  induction 1.
+  exists 1 ; apply tposrp_n_tposr ; auto.
+  destruct_exists.
+  exists (x0 + x).
+  apply tposrp_n_transitive with X ; auto.
+Qed. 
 
-  (* Abs *)
-  intros P B0 Hr.
-  pose (generation_lambda Hr) ; destruct_exists.
-  assert(n0 < x) ; try rewrite <- H6 ; auto with arith.
-  pose (IH _ H15 _ _ _ _ _ H _ _ H7) ; destruct_exists.
-  assert(p < x) ; try rewrite <- H6 ; auto with arith.
-  pose (IH _ H20 _ _ _ _ _ H1 _ _ H9) ; destruct_exists.
-  assert(conv_in_env (A0 :: G) (A' :: G)).
-  apply conv_env_hd with s1 ; auto with coc.
-  apply tposr_eq_tposr ; apply (fromd H).
-  assert(conv_in_env (A0 :: G) (a :: G)).
-  apply conv_env_hd with b ; auto with coc.
-  apply tposr_eq_tposr ; apply (fromd H7).
-  rewrite H13.
-  exists (Abs_l x0 x1) ; intuition ; try apply tposr_abs with s1 ; 
-  try apply tposr_abs with b ; auto with coc.
+Corollary tposrp_cr : 
+  forall e A B T, tposrp e A B T -> forall C, tposrp e A C T -> 
+  exists D, tposrp e B D T /\ tposrp e C D T.
+Proof.
+  intros.
+  pose (tposrp_tposrp_n H).
+  pose (tposrp_tposrp_n H0).
+  destruct_exists.
+  pose (tposrp_n_cr H2 H1).
+  destruct_exists.
+  exists x1.
+  split ; [apply tposrp_n_tposrp with x | apply tposrp_n_tposrp with x0] ; auto.
+Qed.
 
-  apply tposr_exp with (Prod_l A' B) s2 ; auto with coc.
-  apply tposr_abs with s1 B' s2 ; auto with coc.
-  apply conv_env with (A0 :: G) ; auto with coc.
-  apply (fromd H0).
-  apply conv_env with (A0 :: G) ; auto with coc.
-  apply tposr_prod with s1 ; auto with coc.
-  apply (fromd H).
-  apply (left_refl (fromd H0)).
+Corollary tposr_eq_cr : forall e A B s, e |-- A ~= B : s -> 
+  exists C, tposrp e A C (Srt_l s) /\ tposrp e B C (Srt_l s).
+Proof.
+  induction 1.
+  pose (church_rosser H (left_refl H)) ; destruct_exists.
+  exists x ; intuition ; auto with coc.
 
-  apply tposr_equiv_r with (Prod_l A0 a1) ; auto.
-  apply tposr_exp with (Prod_l A' a1) b0 ; auto with coc.
-  apply tposr_abs with b b1 b0 ; auto with coc.
-  apply conv_env with (A0 :: G) ; auto with coc.
-  apply (fromd H11).
-  apply conv_env with (A0 :: G) ; auto with coc.
-  apply tposr_prod with s1 ; auto with coc.
-  apply (fromd H).
-  apply (left_refl (fromd H11)).
+  destruct_exists.
+  exists x ; intuition.
 
-  apply tposr_exp with (Prod_l a B) s2 ; auto with coc.
-  apply tposr_abs with s1 B' s2 ; auto with coc.
-  apply conv_env with (A0 :: G) ; auto with coc.
-  apply (fromd H0).
-  apply conv_env with (A0 :: G) ; auto with coc.
-  apply tposr_prod with b ; auto with coc.
-  apply (fromd H7).
-  apply (left_refl (fromd H0)).
+  destruct_exists.
+  pose (tposrp_cr H4 H1) ; destruct_exists.
+  exists x1 ; intuition.
+  apply tposrp_trans with x0 ; auto with coc.
+  apply tposrp_trans with x ; auto with coc.
+Qed.
 
-  apply tposr_equiv_r with (Prod_l A0 a1) ; auto.
-  apply tposr_exp with (Prod_l a a1) b0 ; auto with coc.
-  apply tposr_abs with b b1 b0 ; auto with coc.
-  apply conv_env with (A0 :: G) ; auto with coc.
-  apply (fromd H11).
-  apply conv_env with (A0 :: G) ; auto with coc.
-  apply tposr_prod with b ; auto with coc.
-  apply (fromd H7).
-  apply (left_refl (fromd H11)).
-
-  (* App *)
-  intros P B0 Hr.
-  pose (generation_app Hr) ; destruct_exists.
-
-  assert(q < x) ; try rewrite <- H7 ; auto with arith.
-  pose (IH _ H16 _ _ _ _ _ H2 _ _ H12) ; destruct_exists.
-  pose (uniqueness_of_types (toq H2) (toq H12)).
-  assert(c = s1).
-  destruct e0 ; destruct_exists.
-  rewrite <- H21 in H8.
-  apply (tposrd_unique_sort H8 H).
-  destruct (conv_refls H21).
-  rewrite <- (tposr_unique_sort H22 (fromd H)).
-  rewrite <- (tposr_unique_sort H23 (fromd H8)).
-  reflexivity.
-
-  assert(A0 :: G |-- B -> a0 : Srt_l b0).
-  apply conv_env with (a :: G) ; auto with coc.
-  apply (fromd H10).
-  destruct e0.
-  rewrite H22.
-  apply conv_env_hd with c.
-  apply tposr_eq_tposr.
-  apply (left_refl (fromd H8)).
-  destruct H22.
-  apply conv_env_hd with x1 ; auto with coc.
-
-  assert(a :: G |-- B -> B' : Srt_l s2).
-  apply conv_env with (A0 :: G) ; auto with coc.
-  apply (fromd H0).
-  destruct e0.
-  rewrite H23.
-  apply conv_env_hd with c.
-  apply tposr_eq_tposr.
-  apply (left_refl (fromd H8)).
-  destruct H23.
-  apply conv_env_hd with x1 ; auto with coc.
-
-  assert(b0 = s2).
-  pose (left_refl H22).
-  pose (left_refl (fromd H0)).
-  apply (tposr_unique_sort t t0).
-  rewrite H21 in H8.
-  rewrite H24 in H10.
-  rewrite H24 in H22.
-  rewrite H24 in H14.
-
-  assert(m0 < x) by rewrite <- H7 ; auto with arith. 
-  pose (tod H22) ; destruct_exists.
-  pose (IH _ H25 _ _ _ _ _ H0 _ _ H26) ; destruct_exists.
-
-  assert(G |-- lsubst x0 x2 ~= lsubst N0 B : s2).
-  apply tposr_eq_sym.
-  apply tposr_eq_trans with (lsubst a1 a0).
-  apply tposr_eq_tposr.
-  change (Srt_l s2) with (lsubst N0 (Srt_l s2)).
-  apply substitution with A0 ; auto with coc.
-  pose (right_refl (fromd H12)).
-  pose (left_refl H19).
-  pose (tposr_uniqueness_of_types t t0).
-  apply tposr_equiv_l with a ; auto with coc.
-  apply (fromd H12).
-
-  apply tposr_eq_tposr.
-  change (Srt_l s2) with (lsubst a1 (Srt_l s2)).
-  apply substitution with A0 ; auto with coc.
-
-  assert(HeqB: equiv G B0 (lsubst N0 B)).
-  right ; exists s2 ; assumption.
-
-  destruct H15 ; destruct_exists.
-
-  (* App, App *)
-  rewrite H33.
-  assert(p < x) ; try rewrite <- H7 ; auto with arith.
-  pose (IH _ H34 _ _ _ _ _ H1 _ _ H15) ; destruct_exists.
-  
-  assert(G |-- App_l B' M' N' -> App_l x2 x3 x0 : lsubst N0 B).
-
-  apply tposr_conv_l with (lsubst N' B') s2 ; auto with coc.
-  apply tposr_eq_trans with (lsubst x0 x2) ; auto with coc.
-  apply tposr_eq_tposr.
-  change (Srt_l s2) with (lsubst N' (Srt_l s2)).
-  apply substitution with A0 ; auto with coc.
-
-  apply tposr_app with A0 A' s1 s2 ; auto with coc.
-  apply (fromd H).
-  apply tposr_conv_l with (Prod_l A0 B) s2 ; auto with coc.
-  apply tposr_eq_tposr.
-  apply tposr_prod with s1 ; auto with coc.
-  apply (left_refl (fromd H)).
-  apply (fromd H0).
-
-  assert(G |-- App_l a0 a2 a1 -> App_l x2 x3 x0 : lsubst N0 B).
-
-  apply tposr_conv_l with (lsubst a1 a0) s2 ; auto with coc.
-  apply tposr_eq_trans with (lsubst x0 x2) ; auto with coc.
-  apply tposr_eq_tposr.
-  change (Srt_l s2) with (lsubst a1 (Srt_l s2)).
-  apply substitution with A0 ; auto with coc.
-
-  apply tposr_app with A0 A' s1 s2 ; auto with coc.
-  apply (fromd H).
-  apply tposr_conv_l with (Prod_l A0 B) s2 ; auto with coc.
-  apply tposr_eq_tposr.
-  apply tposr_prod with s1 ; auto with coc.
-  apply (left_refl (fromd H)).
-
-  exists (App_l x2 x3 x0) ; intuition ; auto with coc.
-  apply tposr_equiv_r with (lsubst N0 B) ; auto with coc.
-  apply tposr_equiv_r with (lsubst N0 B) ; auto with coc.
-
-  (* App, Beta *)
-  rewrite H34.
-  rewrite H15 in H1.
-  pose (generation_lambda H1) ; destruct_exists.
-  assert(c3 < x).
-  rewrite <- H7 ; auto with arith.
-  apply lt_trans with p ; auto with arith.
-  pose (IH _ H43 _ _ _ _ _ H37 _ _ H32) ; destruct_exists.
-  assert(c2 < x).
-  rewrite <- H7 ; auto with arith.
-  apply lt_trans with p ; auto with arith.
-  pose (IH _ H48 _ _ _ _ _ H35 _ _ H8) ; destruct_exists.
-
-  assert(G |-- a ~= a3 : b3).
-  apply tposr_eq_tposr ; auto with coc.
-  apply (fromd H35).
-  assert (conv_in_env (a :: G) (a3 :: G)).
-  apply conv_env_hd with b3 ; auto.
-
-  assert (conv_in_env (A0 :: G) (a3 :: G)).
-  destruct e0.
-  rewrite H55.
-  apply H54.
-  destruct H55.
-  apply conv_env_hd with x5.
-  apply tposr_eq_trans with a ; auto with coc.
-  apply tposr_eq_tposr.
-  destruct (conv_refls H55).
-  pose (tposr_unique_sort H57 (fromd H35)).
-  rewrite e0 ; auto.
-  apply (fromd H35).
-
-  exists (lsubst x0 x3).
-
-  assert(G |-- App_l B' M' N' -> lsubst x0 x3 : lsubst N0 B).
-
-  apply tposr_conv_l with (lsubst N' B') s2 ; auto with coc.
-  apply tposr_eq_trans with (lsubst x0 x2) ; auto with coc.
-  apply tposr_eq_tposr.
-  change (Srt_l s2) with (lsubst N' (Srt_l s2)).
-  apply substitution with A0 ; auto with coc.
-  
-  rewrite H41.
-  apply tposr_beta with x4 s1 x2 s2 ; auto with coc.
-  apply conv_env with (A0 :: G) ; auto with coc.
-  apply conv_env with (a :: G) ; auto with coc.
-  apply tposr_red with B s2 ; auto with coc.
-  apply tposr_conv_l with a b3 ; auto with coc.
-
-  assert(G |-- lsubst a1 b2 -> lsubst x0 x3 : lsubst N0 B).
-
-  apply tposr_conv_l with (lsubst a1 B') s2 ; auto with coc.
-  apply tposr_eq_trans with (lsubst x0 x2) ; auto with coc.
-  apply tposr_eq_tposr.
-  change (Srt_l s2) with (lsubst a1 (Srt_l s2)).
-  apply substitution with A0 ; auto with coc.
-  apply substitution with a ; auto with coc.
-  apply tposr_red with B s2 ; auto with coc.
-
-  intuition ; auto with coc.
-
-  apply tposr_equiv_r with (lsubst N0 B) ; auto.
-  apply tposr_equiv_r with (lsubst N0 B) ; auto.
-
-  (* Beta *)
-  intros P B0 Hr.
-  pose (generation_app Hr) ; destruct_exists.
-
-  assert(q < x) ; try rewrite <- H7 ; auto with arith.
-  pose (IH _ H16 _ _ _ _ _ H2 _ _ H12) ; destruct_exists.
-  pose (uniqueness_of_types (toq H2) (toq H12)).
-  assert(c = s1).
-  destruct e0 ; destruct_exists.
-  rewrite <- H21 in H8.
-  apply (tposrd_unique_sort H8 H).
-  destruct (conv_refls H21).
-  rewrite <- (tposr_unique_sort H22 (fromd H)).
-  rewrite <- (tposr_unique_sort H23 (fromd H8)).
-  reflexivity.
-
-  assert(A0 :: G |-- B -> a0 : Srt_l b0).
-  apply conv_env with (a :: G) ; auto with coc.
-  apply (fromd H10).
-  destruct e0.
-  rewrite H22.
-  apply conv_env_hd with c.
-  apply tposr_eq_tposr.
-  apply (left_refl (fromd H8)).
-  destruct H22.
-  apply conv_env_hd with x1 ; auto with coc.
-
-  assert(a :: G |-- B -> B' : Srt_l s2).
-  apply conv_env with (A0 :: G) ; auto with coc.
-  apply (fromd H0).
-  destruct e0.
-  rewrite H23.
-  apply conv_env_hd with c.
-  apply tposr_eq_tposr.
-  apply (left_refl (fromd H8)).
-  destruct H23.
-  apply conv_env_hd with x1 ; auto with coc.
-
-  assert(b0 = s2).
-  pose (left_refl H22).
-  pose (left_refl (fromd H0)).
-  apply (tposr_unique_sort t t0).
-  rewrite H21 in H8.
-  rewrite H24 in H10.
-  rewrite H24 in H22.
-  rewrite H24 in H14.
-
-  assert(m0 < x) by rewrite <- H7 ; auto with arith. 
-  pose (tod H22) ; destruct_exists.
-  pose (IH _ H25 _ _ _ _ _ H0 _ _ H26) ; destruct_exists.
-
-  assert(G |-- lsubst x0 x2 ~= lsubst N0 B : s2).
-  apply tposr_eq_sym.
-  apply tposr_eq_trans with (lsubst a1 a0).
-  apply tposr_eq_tposr.
-  change (Srt_l s2) with (lsubst N0 (Srt_l s2)).
-  apply substitution with A0 ; auto with coc.
-  pose (right_refl (fromd H12)).
-  pose (left_refl H19).
-  pose (tposr_uniqueness_of_types t t0).
-  apply tposr_equiv_l with a ; auto with coc.
-  apply (fromd H12).
-
-  apply tposr_eq_tposr.
-  change (Srt_l s2) with (lsubst a1 (Srt_l s2)).
-  apply substitution with A0 ; auto with coc.
-
-  assert(HeqB: equiv G B0 (lsubst N0 B)).
-  right ; exists s2 ; assumption.
-
-  destruct H15 ; destruct_exists.
-
-  (* Beta, App *)
-  rewrite H33.
-  pose (generation_lambda H15) ; destruct_exists.
-  assert(p < x).
-  rewrite <- H7 ; auto with arith.
-  pose (IH _ H42 _ _ _ _ _ H1 _ _ H36) ; destruct_exists.
-  assert(n0 < x).
-  rewrite <- H7 ; auto with arith.
-  pose (IH _ H47 _ _ _ _ _ H _ _ H34) ; destruct_exists.
-
-  assert(G |-- A0 ~= a3 : b3).
-  apply tposr_eq_tposr ; auto with coc.
-  apply (fromd H34).
-  assert (conv_in_env (A0 :: G) (a3 :: G)).
-  apply conv_env_hd with b3 ; auto.
-
-  assert (conv_in_env (a :: G) (a3 :: G)).
-  destruct e0.
-  rewrite <- H54.
-  apply H53.
-  destruct H54.
-  apply conv_env_hd with x5.
-  apply tposr_eq_trans with A0 ; auto with coc.
-  apply tposr_eq_tposr.
-  destruct (conv_refls H54).
-  pose (tposr_unique_sort H55 (fromd H34)).
-  rewrite e0 ; auto.
-  apply (fromd H34).
-
-  exists (lsubst x0 x3).
-
-  assert(G |-- App_l a0 a2 a1 -> lsubst x0 x3 : lsubst N0 B).
-
-  apply tposr_conv_l with (lsubst a1 a0) s2 ; auto with coc.
-  apply tposr_eq_trans with (lsubst x0 x2) ; auto with coc.
-  apply tposr_eq_tposr.
-  change (Srt_l s2) with (lsubst a1 (Srt_l s2)).
-  apply substitution with A0 ; auto with coc.
-  
-  rewrite H40.
-  apply tposr_beta with x4 s1 x2 s2 ; auto with coc.
-  apply conv_env with (A0 :: G) ; auto with coc.
-  apply conv_env with (A0 :: G) ; auto with coc.
-  apply tposr_red with B s2 ; auto with coc.
-  apply tposr_conv_l with A0 b3 ; auto with coc.
-
-  assert(G |-- lsubst N' M' -> lsubst x0 x3 : lsubst N0 B).
-
-  apply tposr_conv_l with (lsubst N' a0) s2 ; auto with coc.
-  apply tposr_eq_trans with (lsubst x0 x2) ; auto with coc.
-  apply tposr_eq_tposr.
-  change (Srt_l s2) with (lsubst N' (Srt_l s2)).
-  apply substitution with A0 ; auto with coc.
-  apply substitution with A0 ; auto with coc.
-  apply tposr_red with B s2 ; auto with coc.
-
-  intuition ; auto with coc.
-
-  apply tposr_equiv_r with (lsubst N0 B) ; auto.
-  apply tposr_equiv_r with (lsubst N0 B) ; auto.
-
-  (* Beta, Beta *)
-  rewrite H34.
-  assert(p < x) ; try rewrite <- H7 ; auto with arith.
-  inversion H15.
-  rewrite <- H38 in H32.
-
-  assert(conv_in_env (a :: G) (A0 :: G)).
-  destruct e0.
-  rewrite H36.
-  apply conv_env_hd with s1.
-  apply tposr_eq_tposr.
-  apply (left_refl (fromd H8)).
-  destruct H36.
-  apply conv_env_hd with x3 ; auto with coc.
-
-  assert(A0 :: G |-- M0 -> b2 : B).
-  apply conv_env with (a :: G) ; auto with coc core.
-  apply (fromd H32).
-  
-  pose (tod H39) ; destruct_exists.
-  pose (IH _ H35 _ _ _ _ _ H1 _ _ H40) ; destruct_exists.
-  
-  exists (lsubst x0 x4).
-
-  assert(G |-- lsubst N' M' -> lsubst x0 x4 : lsubst N0 B).
-  apply tposr_conv_l with (lsubst N' B') s2 ; auto with coc.
-  apply tposr_eq_trans with (lsubst x0 x2) ; auto with coc.
-  apply tposr_eq_tposr.
-  change (Srt_l s2) with (lsubst N' (Srt_l s2)).
-  apply substitution with A0 ; auto with coc.
-  apply substitution with A0 ; auto with coc.
-  apply tposr_red with B s2 ; auto with coc.
-  apply conv_env with (a :: G) ; auto with coc.
-
-  assert(G |-- lsubst a1 b2 -> lsubst x0 x4 : lsubst N0 B).
-  apply tposr_conv_l with (lsubst a1 B') s2 ; auto with coc.
-  apply tposr_eq_trans with (lsubst x0 x2) ; auto with coc.
-  apply tposr_eq_tposr.
-  change (Srt_l s2) with (lsubst a1 (Srt_l s2)).
-  apply substitution with A0 ; auto with coc.
-  apply substitution with A0 ; auto with coc.
-  apply tposr_red with B s2 ; auto with coc.
-  apply conv_env with (a :: G) ; auto with coc.
-
+Lemma tposrp_sort_aux : forall e T T' s', tposrp e T T' s' -> forall s, T = Srt_l s -> T' = Srt_l s.
+Proof.
+  induction 1 ; intros.
+  rewrite H0 in H.
+  pose (generation_sort H).
   intuition.
 
-  apply tposr_equiv_r with (lsubst N0 B) ; auto with coc.
-  apply tposr_equiv_r with (lsubst N0 B) ; auto with coc.
+  pose (IHtposrp1 _ H1).
+  apply (IHtposrp2 _ e0).
+Qed.
 
-  (* Red *)
+Lemma tposrp_sort : forall e s T' s', tposrp e (Srt_l s) T' s' -> T' = Srt_l s.
+Proof.
   intros.
-  assert(n0 < x) by rewrite <- H5 ; auto with arith.
-  pose (IH _ H7 _ _ _ _ _ H _ _ H6) ; destruct_exists.
-  exists x0 ; intuition.
-  apply tposr_red with A0 s ; auto with coc.
-  apply (fromd H0).
-  apply tposr_red with A0 s ; auto with coc.
-  apply (fromd H0).
+  apply (tposrp_sort_aux H) ; auto.
+Qed.
 
-  (* Exp *)
-  intros.
-  assert(n0 < x) by rewrite <- H5 ; auto with arith.
-  pose (IH _ H7 _ _ _ _ _ H _ _ H6) ; destruct_exists.
-  exists x0 ; intuition.
-  apply tposr_exp with B s ; auto with coc.
-  apply (fromd H0).
-  apply tposr_exp with B s ; auto with coc.
-  apply (fromd H0).
-  
-  (* Subset *)
-  intros.
-  pose (generation_subset H6) ; destruct_exists.
-  rewrite H11.
+Lemma equiv_sort_eq : forall e s s0, equiv e (Srt_l s) (Srt_l s0) -> s = s0.
+Proof.
+   intros.
+   destruct H.
+   inversion H ; auto.
+   destruct H.
+   pose (tposr_eq_cr H) ; destruct_exists.
+   pose (tposrp_sort H0).
+   pose (tposrp_sort H1).
+   rewrite e0 in e1.
+   inversion e1 ; auto.
+Qed.   
 
-  assert(n0 < x) by rewrite <- H5 ; auto with arith.
-  assert(m0 < x) by rewrite <- H5 ; auto with arith.
-  pose (IH _ H13 _ _ _ _ _ H _ _ H7) ; destruct_exists.
-  pose (IH _ H14 _ _ _ _ _ H0 _ _ H9) ; destruct_exists.
+Lemma tposrp_left_refl : forall e A B T, tposrp e A B T -> e |-- A -> A : T.
+Proof.
+  induction 1 ; auto with coc.
+  apply (left_refl H).
+Qed.
 
-  assert(conv_in_env (A0 :: G) (a :: G)).
-  apply conv_env_hd with set ; auto with coc.
-  apply tposr_eq_tposr.
-  apply (fromd H7).
+Lemma tposrp_right_refl : forall e A B T, tposrp e A B T -> e |-- B -> B : T.
+Proof.
+  induction 1 ; auto with coc.
+  apply (right_refl H).
+Qed.
 
-  assert(conv_in_env (A0 :: G) (A' :: G)).
-  apply conv_env_hd with set ; auto with coc.
-  apply tposr_eq_tposr.
-  apply (fromd H).
+Lemma tposrp_conv_env : forall e A B T, tposrp e A B T ->
+  forall f, conv_in_env e f -> tposrp f A B T.
+Proof.
+  induction 1 ; intros ; auto with coc.
+  apply tposrp_tposr.
+  apply conv_env with e ; auto with coc.
+  apply tposrp_trans with X ; auto with coc.
+Qed.
 
-  exists (Subset_l x0 x1).
-  assert(G |-- Subset_l A' B' -> Subset_l x0 x1 : Srt_l set).
-  apply tposr_subset ; auto with coc.
-  apply conv_env with (A0 :: G) ; auto.
-
-  assert(G |-- Subset_l a a0 -> Subset_l x0 x1 : Srt_l set).
-  apply tposr_subset ; auto with coc.
-  apply conv_env with (A0 :: G) ; auto.
-  
-  intuition ; try apply tposr_equiv_r with (Srt_l set) ; auto with coc.
-
-  (* Sum *)
-  rewrite <- H2 in Hl2.
-  rewrite <- H3 in Hl2.
-  rewrite <- H4 in Hl2.
-  intros P B0 Hr.
-  pose (generation_sum Hr) ; destruct_exists.
-  rewrite H12.
-
-  assert(n0 < x) by rewrite <- H6 ; auto with arith.
-  pose (IH _ H14 _ _ _ _ _ H _ _ H7) ; destruct_exists.
-  assert(m0 < x) by rewrite <- H6 ; auto with arith.
-  pose (IH _ H19 _ _ _ _ _ H0 _ _ H9) ; destruct_exists.
-
-  assert(conv_in_env (A0 :: G) (A' :: G)).
-  apply conv_env_hd with s1 ; auto with coc.
-  apply tposr_eq_tposr ; apply (fromd H).
-  assert(conv_in_env (A0 :: G) (a :: G)).
-  apply conv_env_hd with b ; auto with coc.
-  apply tposr_eq_tposr ; apply (fromd H7).
-
-  exists (Sum_l x1 x2).
-  assert(G |-- Sum_l A' B' -> Sum_l x1 x2 : Srt_l s3).
-  apply tposr_sum with s1 s2 ; auto with coc.
-  apply conv_env with (A0 :: G) ; auto with coc.
-  assert(G |-- Sum_l A' B' -> Sum_l x1 x2 : Srt_l x0).
-  apply tposr_sum with b b0 ; auto with coc.
-  apply conv_env with (A0 :: G) ; auto with coc.
-  assert(G |-- Sum_l a a0 -> Sum_l x1 x2 : Srt_l s3).
-  apply tposr_sum with s1 s2 ; auto with coc.
-  apply conv_env with (A0 :: G) ; auto with coc.
-  assert(G |-- Sum_l a a0 -> Sum_l x1 x2 : Srt_l x0).
-  apply tposr_sum with b b0 ; auto with coc.
-  apply conv_env with (A0 :: G) ; auto with coc.
-   
-  intuition ; try apply tposr_equiv_r with (Srt_l x0) ; auto.
-
-  (* Pair *)
-  rewrite <- H5 in Hl2.
-  rewrite <- H6 in Hl2.
-  rewrite <- H7 in Hl2.
-  intros P B0 Hr.
-  pose (generation_pair Hr) ; destruct_exists.
-  rewrite H19.
-  inversion H9.
-  rewrite <- H22 in H10.
-  rewrite <- H22 in H20.
-  rewrite <- H22.
-  rewrite <- H22 in H12.
-  rewrite <- H23 in H12.
-  rewrite <- H23 in H17.
-  rewrite <- H23 in H20.
-  rewrite <- H23.
-  rewrite <- H22 in H15.
-  clear H22 H23 H9 a a0.
-
-  assert(n0 < x) by rewrite <- H8 ; auto with arith.
-  pose (IH _ H9 _ _ _ _ _ H _ _ H10) ; destruct_exists ; clear H9.
-  assert(m0 < x) by rewrite <- H8 ; auto with arith.
-  pose (IH _ H9 _ _ _ _ _ H0 _ _ H12) ; destruct_exists ; clear H9.
-  assert(p < x) by rewrite <- H8 ; auto with arith.
-  pose (IH _ H9 _ _ _ _ _ H2 _ _ H15) ; destruct_exists ; clear H9.
-  assert(q < x) by rewrite <- H8 ; auto with arith.
-  pose (IH _ H9 _ _ _ _ _ H3 _ _ H17) ; destruct_exists ; clear H9.
-
-  exists (Pair_l (Sum_l x1 x2) x3 x4).
-
-  assert(conv_in_env (A0 :: G) (A' :: G)).
-  apply conv_env_hd with s1 ; auto with coc.
-  apply tposr_eq_tposr ; apply (fromd H).
-  assert(conv_in_env (A0 :: G) (b :: G)).
-  apply conv_env_hd with c ; auto with coc.
-  apply tposr_eq_tposr ; apply (fromd H10).
-  pose (fromd H).
-  pose (fromd H0).
-  pose (fromd H2).
-  pose (fromd H3).
-  pose (fromd H10).
-  pose (fromd H12).
-  pose (fromd H15).
-  pose (fromd H17).
-
-  assert(G |-- Pair_l (Sum_l A' B') u' v' -> Pair_l (Sum_l x1 x2) x3 x4 : Sum_l A0 B).
-  apply tposr_conv_r with (Sum_l A' B') s3 ; auto with coc ; try apply tposr_pair with s1 s2 s3 ; auto with coc.
-  apply tposr_eq_tposr.
-  apply tposr_sum with s1 s2 ; auto with coc.
-  apply conv_env with (A0 :: G) ; auto with coc.
-  apply tposr_red with A0 s1 ; auto with coc.
-  apply tposr_conv_l with (lsubst u B) s2 ; auto with coc.
-  apply tposr_eq_tposr.
-  change (Srt_l s2) with (lsubst u (Srt_l s2)).
-  apply substitution with A0 ; auto with coc.
-
-  assert(G |-- Pair_l (Sum_l b b0) a1 a2 -> Pair_l (Sum_l x1 x2) x3 x4 : Sum_l A0 B).
-  apply tposr_conv_r with (Sum_l b b0) x0 ; auto with coc ; try apply tposr_pair with c c0 x0 ; auto with coc.
-  apply tposr_eq_tposr.
-  apply tposr_sum with c c0 ; auto with coc.
-  apply conv_env with (A0 :: G) ; auto with coc.
-  apply tposr_red with A0 c ; auto with coc.
-  apply tposr_conv_l with (lsubst u B) c0 ; auto with coc.
-  apply tposr_eq_tposr.
-  change (Srt_l c0) with (lsubst u (Srt_l c0)).
-  apply substitution with A0 ; auto with coc.
-   
-  intuition ; try apply tposr_equiv_r with (Sum_l A0 B) ; auto.
-
-  (* Pi1 *)
-  intros.
-  pose (generation_pi1 H8) ; destruct_exists.
-  inversion H13.
-  rewrite <- H18 in H15.
-  rewrite <- H18 in H16.
-  rewrite <- H18.
-  rewrite <- H19 in H16.
-  clear a1 b1 H19 H18 H13.
-  
-  assert(n0 < x) by rewrite <- H7 ; auto with arith.
-
-  pose (fromd H).
-  pose (fromd H0).
-  pose (fromd H2).
-  pose (fromd H9).
-  pose (fromd H11).
-
-  destruct H16 ; destruct_exists.
-
-  (* Pi1, Pi1 *)
-  rewrite H16 in H9.
-  rewrite H17 in H11.
-  rewrite H16 in H11.
-  rewrite H16 in H19.
-  rewrite H18 in H21.
-  rewrite H16 in t3.
-  rewrite H16 in t4.
-  rewrite H17 in t4.
-  rewrite H17 in H19.
-  rewrite H17 in H24.
-  rewrite H16 in H23.
-  clear a a0 H16 H17 H9 H11.
-
-  pose (IH _ H13 _ _ _ _ _ H _ _ H22) ; destruct_exists ; clear H13.
-  assert(m0 < x) by rewrite <- H7 ; auto with arith.
-  pose (IH _ H13 _ _ _ _ _ H0 _ _ H23) ; destruct_exists ; clear H13.
-  clear H24.
-  assert(p < x) by rewrite <- H7 ; auto with arith.
-  pose (IH _ H13 _ _ _ _ _ H2 _ _ H19) ; destruct_exists ; clear H13.
-
-  assert(conv_in_env (A :: G) (A' :: G)).
-  apply conv_env_hd with s1 ; auto with coc.
-  assert(conv_in_env (A :: G) (b :: G)).
-  apply conv_env_hd with c ; auto with coc.
-
-  exists (Pi1_l (Sum_l x1 x2) x3).
-  assert(G |-- Pi1_l (Sum_l A' B') t' -> Pi1_l (Sum_l x1 x2) x3 : A).
-  apply tposr_conv_r with A' s1 ; auto with coc ; try apply tposr_pi1 with s1 s2 s3 ; auto with coc.
-  apply conv_env with (A :: G) ; auto with coc.
-  apply tposr_red with (Sum_l A B) s3 ; auto with coc.
-  apply tposr_sum with s1 s2 ; auto with coc.
-  
-  rewrite H21.
-  assert(G |-- Pi1_l (Sum_l b b0) b1 -> Pi1_l (Sum_l x1 x2) x3 : A).
-  apply tposr_conv_r with b c ; auto with coc ; try apply tposr_pi1 with c c0 x0 ; auto with coc.
-  apply conv_env with (A :: G) ; auto with coc.
-  apply tposr_red with (Sum_l A B) x0 ; auto with coc.
-  apply tposr_sum with c c0 ; auto with coc.
-   
-  intuition ; try apply tposr_equiv_r with A ; auto.
-  
-  (* Pi1, Pi1_red *)
-  rewrite H21.
-  rewrite H16 in H2.
-  pose (generation_pair H22) ; destruct_exists.
-  rewrite H33.
-  inversion H23.
-  rewrite <- H36 in H24.
-  rewrite <- H36 in H26.
-  rewrite <- H36 in H29.
-  rewrite <- H36 in H34.
-  rewrite <- H37 in H26.
-  rewrite <- H37 in H31.
-  rewrite <- H37 in H34.
-  clear H36 H37 a3 a4 H23.
-  rewrite H16 in H19.
-  pose (generation_pair H19) ; destruct_exists.
-  inversion H23.
-  rewrite <- H47 in H35.
-  rewrite <- H47 in H37.
-  rewrite <- H47 in H40.
-  rewrite <- H47 in H45.
-  rewrite <- H48 in H37.
-  rewrite <- H48 in H42.
-  rewrite <- H48 in H45.
-  clear H47 H48 a3 a4 H23.
- 
-  assert(d1 < x) by rewrite <- H7 ; apply lt_trans with p ;  auto with arith.
-  pose (IH _ H23 _ _ _ _ _ H24 _ _ H35) ; destruct_exists ; clear H23.
-  assert(d2 < x) by rewrite <- H7 ; apply lt_trans with p ; auto with arith.
-  pose (IH _ H23 _ _ _ _ _ H26 _ _ H37) ; destruct_exists ; clear H23.
-  assert(b5 < x) by rewrite <- H7 ; apply lt_trans with p ; auto with arith.
-  pose (IH _ H23 _ _ _ _ _ H29 _ _ H40) ; destruct_exists ; clear H23.
-  assert(b6 < x) by rewrite <- H7 ; apply lt_trans with p ; auto with arith.
-  pose (IH _ H23 _ _ _ _ _ H31 _ _ H42) ; destruct_exists ; clear H23.
-
-  pose (fromd H24).
-  assert(conv_in_env (a :: G) (b3 :: G)).
-  apply conv_env_hd with c2 ; apply tposr_eq_tposr ; apply t5.
-  assert(conv_in_env (a :: G) (A :: G)).
-  apply conv_env_hd with c ; auto with coc.
-  assert(convAA':conv_in_env (A :: G) (A' :: G)).
-  apply conv_env_hd with s1 ; auto with coc.
-
-  destruct (conv_refls H17).
-  destruct (conv_refls H18).
-  assert(s1 = c).
-  apply (tposr_unique_sort t0 H63).
-  pose (tposr_unique_sort t5 H64).
-  assert(s2 = c0).
-  pose (fromd H0).
-  apply (tposr_unique_sort t6 H65).
-
-  exists x5.
-  assert(G |-- Pi1_l (Sum_l A' B') (Pair_l (Sum_l b3 b4) a5 a6) -> x5 : A).
-  apply tposr_conv_r with A' s1 ; auto with coc.
-  apply tposr_pi1_red with x3 c2 x4 c3 x1 x6 ; auto with coc.
-  apply conv_env with (a :: G) ; auto with coc.
-  apply tposr_pair with c2 c3 x1 ; auto with coc.
-  apply conv_env with (a :: G) ; auto with coc.
-  apply tposr_red with a c2 ; auto.
-  apply tposr_conv_l with (lsubst a1 a0) c3; auto with coc.
-  apply tposr_eq_tposr.
-  change (Srt_l c3) with (lsubst a1 (Srt_l c3)).
-  apply substitution with a ; auto with coc.
-  apply (fromd H26).
-  apply (fromd H29).
-
-  apply tposr_eq_trans with A.
-  apply tposr_eq_sym.
-  apply tposr_eq_tposr.
-  rewrite e0.
-  rewrite <- H67 ; auto.
-  apply tposr_eq_trans with a ; auto with coc.
-  rewrite e0 ; auto.
-
-  apply tposr_eq_trans with B.
-  apply tposr_eq_sym.
-  apply tposr_eq_tposr.
-  assert(c0 = c3).
-  pose(fromd H26).
-  assert(A :: G |-- a0 -> b4 : Srt_l c3).
-  apply conv_env with (a :: G) ; auto with coc.
-  apply (tposr_unique_sort H66 H69).
-  rewrite <- H69.
-  rewrite <- H68 ; auto.
-  apply conv_env with (A :: G) ; auto with coc.
-  apply tposr_eq_trans with a0 ; auto with coc.
-  assert(c3 = c0).
-  assert(A :: G |-- a0 -> b4 : Srt_l c3).
-  apply conv_env with (a :: G) ; auto with coc.
-  apply (fromd H26).
-  apply (tposr_unique_sort H69 H66).
-  rewrite H69.
-  apply conv_env_eq with (A :: G) ; auto with coc.
-  apply tposr_eq_tposr.
-  apply conv_env with (a :: G) ; auto with coc.
-  apply (fromd H26).
-  apply conv_env_hd with c ; auto with coc.
-  apply tposr_eq_trans with A ; auto with coc.
-  rewrite <- H67.
-  apply tposr_eq_tposr.
-  apply (fromd H).
-  
-  assert(G |-- b1 -> x5 : A).
-  inversion H44.
-  apply tposr_conv_l with a c ; auto with coc.
-
-  intuition ; try apply tposr_equiv_r with A ; auto.
-
-  (* Pi1_red *)
-  intros.
-  rewrite <- H7.
-  rewrite H8 in H6.
-  clear H8 A''.
-  pose (generation_pair H2) ; destruct_exists.
-  inversion H8.
-  generalize dependent G.
-  rewrite <- H23 ; rewrite <- H24.
-  inversion H20.
-  rewrite <- H0 ; rewrite <- H2.
-  rewrite <- H3 ; rewrite <- H4.
-  clear a a0 H8 H23 H24 H0 H2 H3 H4 b b0 a1 a2 H20 ; intros.
-  clear e H5.
-
-  pose (generation_pi1 H10) ; destruct_exists.
-  inversion H23.
-  generalize dependent G.
-  rewrite <- H28.
-  rewrite <- H29.
-  clear H23 H29 H28 a1 b3.
-  intros.
-
-  assert(s1 = c).
-  apply (tposr_unique_sort (fromd H) (fromd H11)).
-  
-  assert(s2 = c0).
-  apply (tposr_unique_sort (fromd H0) (fromd H13)).
-  generalize dependent G.
-  rewrite <- H23.
-  rewrite <- H27.
-  intros.
-  
-  destruct H26 ; destruct_exists.
-  
-  (* Pi1_red, Pi1 *)
-  generalize dependent G.
-  rewrite H26.
-  rewrite H28.
-  rewrite H32.
-  rewrite H29.
-  clear a a0 a1 P H26 H28 H29 H32.
-  intros.
-  pose (generation_pair H30).
-  destruct_exists.
-  inversion H26.
-  generalize dependent G.
-  rewrite <- H42.
-  rewrite <- H43.
-  clear H42 H43 H26 a a0.
-  rewrite H39.
-  rewrite <- H6.
-  rewrite <- H7.
-  intros.
-
-  assert(b1 < x) by rewrite <- H9 ; apply lt_trans with p ; auto with arith.
-  pose (IH _ H26 _ _ _ _ _ H16 _ _ H35) ; destruct_exists.
-  exists x3.
-  
-  assert(G |-- u' -> x3 : A).
-  apply tposr_conv_l with A0 s1; auto with coc.
-  
-  assert(conv_in_env (A0 :: G) (b4 :: G)).
-  apply conv_env_hd with c4 ; apply tposr_eq_tposr ; apply (fromd H28).
-
-  pose (conv_refls H3) ; destruct_exists.
-  pose (tposr_unique_sort H47 (fromd H5)).
-  pose (tposr_unique_sort H48 (left_refl (fromd H28))).
-
-  assert(G |-- b ~= b4 : c4).
-  apply tposr_eq_trans with A0 ; auto with coc.
-  apply tposr_eq_trans with A ; auto with coc.
-  apply tposr_eq_sym.
-  apply tposr_eq_tposr.
-  rewrite <- e0.
-  rewrite e ; apply (fromd H5).
-  rewrite <- e0.
-  assumption.
-  apply tposr_eq_tposr ; apply (fromd H28).
-
-  pose (conv_refls H4) ; destruct_exists.
-  assert(c2 = s2).
-  apply (tposr_unique_sort (fromd H20) H50).
-
-  assert(conv_in_env (A0 :: G) (A :: G)).
-  apply conv_env_hd with s1 ; auto with coc.
-  assert(A :: G |-- B -> b5 : Srt_l c5).
-  apply conv_env with (A0 :: G) ; auto.
-  apply (fromd H32).
-
-  assert(c5 = s2).
-  apply (tposr_unique_sort H54 H51).
-  assert(s1 = c1) ; auto.
-  assert(s1 = c4) ; auto.
-  generalize dependent G.
-  rewrite H52.
-  rewrite H55.
-  rewrite <- H56.
-  rewrite <- H57.
-  clear H52 H55 H56 H57.
-  intros.
-
-  assert(A :: G |-- b0 ~= b5 : s2).
-  apply tposr_eq_trans with B ; auto.
-  apply tposr_eq_trans with B'' ; auto with coc.
-  apply tposr_eq_sym.
-  apply tposr_eq_tposr.
-  apply (fromd H20).
+Lemma tposrp_tposr_eq_aux : forall e A B T, tposrp e A B T -> forall s, T = Srt_l s -> e |-- A ~= B : s.
+Proof.
+  induction 1 ; simpl ; intros ; auto with coc.
+  rewrite H0 in H.
   apply tposr_eq_tposr ; auto.
+  apply tposr_eq_trans with X ; auto with coc.
+Qed.
 
-  assert(G |-- Pi1_l (Sum_l b b0) (Pair_l (Sum_l b4 b5) a1 a2) -> x3 : A).
-  apply tposr_exp with b s1 ; try apply (fromd H5) ; auto with coc.
-  apply tposr_pi1_red with b4 s1 b5 s2 s3 a2 ; auto with coc.
-  apply (right_refl (fromd H28)).
-  apply conv_env with (A0 :: G) ; auto with coc.
-  apply (right_refl (fromd H32)).
-  apply tposr_pair with s1 s2 s3; auto with coc.
-  apply (right_refl (fromd H28)).
-  apply conv_env with (A0 :: G) ; auto with coc.
-  apply (right_refl (fromd H32)).
-  apply tposr_conv_l with A0 s1 ; auto.
-  apply tposr_eq_tposr ; apply (fromd H28).
-  apply tposr_conv_l with (lsubst u B) s2 ; auto with coc.
-  apply tposr_eq_tposr.
-  change (Srt_l s2) with (lsubst u (Srt_l s2)).
-  apply substitution with A0 ; auto with coc.
-  apply (fromd H32).
-  apply (fromd H35).
-  apply (right_refl (fromd H37)).
-  apply conv_env_eq with (A :: G) ; auto with coc.
-  apply conv_env_hd with s1 ; apply tposr_eq_tposr ; apply (fromd H5).
+Lemma tposrp_tposr_eq : forall e A B s, tposrp e A B (Srt_l s) -> e |-- A ~= B : s.
+Proof.
+  intros ; apply tposrp_tposr_eq_aux with (Srt_l s) ; auto.
+Qed.
 
-  intuition ; try apply tposr_equiv_r with A ; auto.
-
-  (* Pi1_red, Pi1_red *)
-  rewrite H32.
-  generalize dependent G.
-  rewrite <- H7.
-  clear H23 H27.
-  inversion H26.
-  rewrite <- H0.
-  rewrite <- H2.
-  rewrite <- H3.
-  rewrite <- H4.
-  clear H0 H2 H3 H4 H26.
-  intros.
+Lemma tposrp_pi_aux : forall e T T' Ts, tposrp e T T' Ts -> 
+  forall A B, T = Prod_l A B -> forall s, Ts  = Srt_l s -> exists3 A' B' s1, T' = Prod_l A' B' /\
+  tposrp e A A' (Srt_l s1) /\ tposrp (A :: e) B B' (Srt_l s).
+Proof.
+  induction 1 ; simpl ; intros.
   
-  pose (generation_pair H2).
-  pose (generation_pair H30).
-  destruct_exists.
-  generalize dependent G.
-  inversion H26 ; inversion H23.
-  rewrite <- H0.
-  rewrite <- H2.
-  rewrite <- H3.
-  rewrite <- H4.
-  clear H0 H2 H3 H4 H26 H23.
-  inversion H52.
-  rewrite <- H0.
-  rewrite <- H2.
-  rewrite <- H3.
-  rewrite <- H4.
-  clear H0 H2 H3 H4 H52.
-  inversion H41.
-  rewrite <- H0.
-  rewrite <- H2.
-  rewrite <- H3.
-  rewrite <- H4.
-  clear H0 H2 H3 H4 H41.
+  rewrite H0 in H.
+  rewrite H1 in H.
+  pose (tod H) ; destruct_exists.
+  pose (generation_prod H2) ; destruct_exists.
+  exists a a0 b ; intuition ; try apply tposrp_tposr ; auto.
+  apply (fromd H3).
+  rewrite (equiv_sort_eq H8).
+  apply (fromd H5).
+    
+  pose (IHtposrp1 _ _ H1 _ H2) ; destruct_exists.
+  pose (IHtposrp2 _ _ H3 _ H2) ; destruct_exists.
+  exists a0 b0 c0 ; intuition ; auto with coc.
+  apply tposrp_trans with a ; auto with coc.
+  pose (tposrp_left_refl H7).
+  pose (tposrp_right_refl H4).
+  rewrite (tposr_unique_sort t t0).
+  assumption.
+  apply tposrp_trans with b ; auto with coc.
+  apply tposrp_conv_env with (a :: e) ; auto with coc. 
+  apply conv_env_hd with c ; auto with coc.
+  apply tposr_eq_sym.
+  apply (tposrp_tposr_eq H4).
+Qed.  
+
+Lemma tposrp_pi : forall e A B T s, tposrp e (Prod_l A B) T (Srt_l s) -> 
+  exists3 A' B' s1, T = Prod_l A' B' /\
+  tposrp e A A' (Srt_l s1) /\ tposrp (A :: e) B B' (Srt_l s).
+Proof.
+  intros ; apply tposrp_pi_aux with (Prod_l A B) (Srt_l s) ; auto with coc.
+Qed.
+
+Corollary injectivity_of_pi : forall e A A' B B' s, e |-- Prod_l A B ~= Prod_l A' B' : s ->
+  exists s1, e |-- A ~= A' : s1 /\ A :: e |-- B ~= B' : s.
+Proof.
   intros.
-
-  assert(b1 < x) by rewrite <- H9 ; apply lt_trans with p ; auto with arith.
-  pose (IH _ H23 _ _ _ _ _ H16 _ _ H37) ; destruct_exists.
-  exists x4.
-
-  assert(equiv G A A0).
-  right ; exists s1 ; auto.
-
-  assert(equiv G B0 A0).
-  destruct H55 ; destruct_exists.
-  rewrite <- H55 ; auto.
-  pose (tposr_eq_sym H55).
-  assert(equiv G A0 A) by right ; exists x5 ; auto.
-  apply (equiv_trans H25 H56).
-
-  intuition ; try apply tposr_equiv_r with A0 ; auto.
-
-  (* Pi2 *)
-
-
-
-
-
-
-
-
-
-
-
-
+  pose (tposr_eq_cr H) ; destruct_exists.
+  pose (tposrp_pi H0).
+  pose (tposrp_pi H1).
+  destruct_exists.
+  rewrite H2 in H3.
+  generalize dependent e.
+  inversion_clear H3.
+  intros.
+  pose (tposrp_right_refl H6).
+  pose (tposrp_right_refl H4).
+  pose (tposr_unique_sort t t0).
+  rewrite <- e0 in H4.
+  pose (tposrp_tposr_eq H3).
+  pose (tposrp_tposr_eq H6).
+  pose (tposrp_tposr_eq H7).
+  pose (tposrp_tposr_eq H5).
+  exists c0.
+  assert(e |-- A ~= A' : c0).
+  apply tposr_eq_trans with a0 ; auto with coc.
+  intuition.
+  apply tposr_eq_trans with b0 ; auto with coc.
+  apply conv_env_eq with (A' :: e) ; auto with coc.
+  apply conv_env_hd with c0 ; auto with coc.
+Qed.
