proof/JRussell/Substitution.v
@@ -142,11 +142,11 @@ apply jeq_app with (subst_rec d A n) ; auto with coc.
 rewrite distr_subst.
 rewrite distr_subst.
 apply jeq_beta with s1 s2 ; auto with coc.
-
+(*
 apply jeq_red with (subst_rec d A n) s ; auto with coc.
 
 apply jeq_exp with (subst_rec d B n) s ; auto with coc.
-
+*)
 apply jeq_sum with s1 s2 ; auto with coc.
 
 apply jeq_pair with s1 s2 s3 ; auto with coc.
